add Church-style judgments

src/hol.lean
@@ -2,7 +2,8 @@
 
 import moromoro
 
-@[derive decidable_eq]
+namespace hol
+
 inductive type : Type
 | base : type
 | prop : type
@@ -11,25 +12,154 @@ open type
 
 variable ν : type → Type
 
-inductive preterm : type → Type
-| var : Π {t}, ν t → preterm t
-| lam : Π {t₁ t₂}, (ν t₁ → preterm t₂) → preterm (arrow t₁ t₂)
-| app : Π {t₁ t₂}, preterm (arrow t₁ t₂) → preterm t₁ → preterm t₂
-| eq : Π {t}, preterm t → preterm t → preterm prop
-open preterm
+inductive term : type → Type
+| var : Π {t}, ν t → term t
+| lam : Π {t₁ t₂}, (ν t₁ → term t₂) → term (arrow t₁ t₂)
+| app : Π {t₁ t₂}, term (arrow t₁ t₂) → term t₁ → term t₂
+| eq : Π {t}, term t → term t → term prop
+open term
 
-def Preterm (t : type) : Type 1 :=
-Π ν, preterm ν t
+def Term (t : type) : Type 1 :=
+Π ν, term ν t
 
-def term : list type → type → Type :=
-λ Γ t, list.foldr (λ t α, ν t → α) (preterm ν t) Γ
+def judgment : list type → type → Type :=
+λ Γ t, list.foldr (λ t α, ν t → α) (term ν t) Γ
 
-def Term (Γ : list type) (t : type) : Type 1 :=
-Π ν, term ν Γ t
+def Judgment (Γ : list type) (t : type) : Type 1 :=
+Π ν, judgment ν Γ t
 
 ----
 
-variables {Γ : list type} {t : type}
+universe u
+variable {α : Type u}
+
+inductive mem : α → list α → Type u
+| here : Π {x l}, mem x (x :: l)
+| there : Π {x l y}, mem x l → mem x (y :: l)
+open mem
+
+local infix ` ∈' `:50 := mem
+
+variables {Γ Γ₁ Γ₂ : list type} {t t₁ t₂ t₃ : type}
+
+def subst' : Π {t : type}, term (term ν) t → term ν t
+| _ (var m) := m
+| _ (lam f) := lam (λ x, subst' (f (var x)))
+| _ (app m₁ m₂) := app (subst' m₁) (subst' m₂)
+| _ (eq m₁ m₂) := eq (subst' m₁) (subst' m₂)
+
+namespace judgment
+  def weak : Judgment Γ t₂ → Judgment (t₁ :: Γ) t₂ :=
+  λ m ν x, m ν
+
+  def var' : Π {Γ}, judgment ν (t :: Γ) t
+  | [] := λ x, var x
+  | (t :: Γ) := λ x y, var' x
+
+  def var : Π {Γ}, t ∈' Γ → Judgment Γ t
+  | _ here := λ ν, var' ν
+  | _ (there h) := weak (var h)
+
+  def lam' : Π {Γ}, judgment ν (t₁ :: Γ) t₂ → judgment ν Γ (arrow t₁ t₂)
+  | [] m := lam (λ x, m x)
+  | (t :: Γ) f := λ x, lam' (λ y, f y x)
+
+  def lam : Judgment (t₁ :: Γ) t₂ → Judgment Γ (arrow t₁ t₂) :=
+  λ m ν, lam' ν (m ν)
+
+  def app' : Π {Γ}, judgment ν Γ (arrow t₁ t₂) → judgment ν Γ t₁ → judgment ν Γ t₂
+  | [] m₁ m₂ := app m₁ m₂
+  | (t :: Γ) f m := λ x, app' (f x) (m x)
+
+  def app : Judgment Γ (arrow t₁ t₂) → Judgment Γ t₁ → Judgment Γ t₂ :=
+  λ m₁ m₂ ν, app' ν (m₁ ν) (m₂ ν)
+
+  def eq' : Π {Γ : list type}, judgment ν Γ t → judgment ν Γ t → judgment ν Γ prop
+  | [] m₁ m₂ := eq m₁ m₂
+  | (t :: Γ) m₁ m₂ := λ x, eq' (m₁ x) (m₂ x)
+
+  def eq : Judgment Γ t → Judgment Γ t → Judgment Γ prop :=
+  λ m₁ m₂ ν, eq' ν (m₁ ν) (m₂ ν)
+
+  def subst''' : Π {Γ}, judgment (term ν) (t₁ :: Γ) t₂ → judgment ν Γ t₁ → judgment ν Γ t₂
+  | [] m₁ m₂ := subst' ν (m₁ m₂)
+  | (t :: Γ) f m := λ x, subst''' (λ x', f x' (term.var x)) (m x)
+
+  def subst : Judgment (t₁ :: Γ) t₂ → Judgment Γ t₁ → Judgment Γ t₂ :=
+  λ m₁ m₂ ν, subst''' ν (m₁ _) (m₂ ν)
+end judgment
+open judgment
+
+----
+
+def type.fold : list type → type → type :=
+λ Γ t, list.foldr arrow t Γ
+
+def judgment.to_term' : Π {Γ : list type}, judgment ν Γ t → term ν (type.fold Γ t)
+| [] m := m
+| (t :: Γ) f := lam (λ x, judgment.to_term' (f x))
+
+def judgment.to_term : Judgment Γ t → Term (type.fold Γ t) :=
+λ m ν, judgment.to_term' ν (m ν)
+
+def term_subst' : term (term ν) (arrow t₁ t₂) → term ν t₁ → term (term ν) t₂
+| (lam f) m := f m
+| m₁ m₂ := app m₁ (var m₂)
+
+def term.to_judgment' : Π {Γ : list type}, term (term ν) (type.fold Γ t) → judgment ν Γ t
+| [] m := subst' ν m
+| (t :: Γ) m := λ x, term.to_judgment' (term_subst' ν m (var x))
+
+def term.to_judgment : Term (type.fold Γ t) → Judgment Γ t :=
+λ m ν, term.to_judgment' ν (m _)
+
+----
+
+def domain : type → Type
+| base := term ν base
+| prop := term ν prop
+| (arrow t₁ t₂) := domain t₁ → domain t₂
+
+def Domain (t : type) : Type 1 :=
+Π ν, domain ν t
+
+def reify_reflect : Π (t : type), (domain ν t → term ν t) × (term ν t → domain ν t)
+| base := ⟨ id, id ⟩
+| prop := ⟨ id, id ⟩
+| (arrow t₁ t₂) :=
+   let r₁ := reify_reflect t₁ in
+   let r₂ := reify_reflect t₂ in
+   let reify (f : domain ν t₁ → domain ν t₂) := lam (λ x, r₂.1 (f (r₁.2 (var x)))) in
+   let reflect (f : term ν (arrow t₁ t₂)) := λ x, r₂.2 (app f (r₁.1 x)) in
+   ⟨reify, reflect⟩
+
+def reify' : domain ν t → term ν t :=
+λ x, (reify_reflect ν t).1 x
+
+def reify : Domain t → Term t :=
+λ x ν, reify' ν (x ν)
+
+def eval' : Π {t : type}, term (domain ν) t → domain ν t
+| _ (var x) := x
+| _ (lam f) := λ x, eval' (f x)
+| _ (app m₁ m₂) := (eval' m₁) (eval' m₂)
+| _ (eq m₁ m₂) := eq (reify' ν (eval' m₁)) (reify' ν (eval' m₂))
+
+def eval : Term t → Domain t :=
+λ m ν, eval' ν (m _)
+
+def normalize : Term t → Term t :=
+reify ∘ eval
+
+instance term_setoid : setoid (Term t) :=
+⟨inv_image eq normalize,
+ inv_image.equivalence eq normalize eq.equivalence⟩
+
+instance judgment_setoid [h : setoid (Term (type.fold Γ t))] : setoid (Judgment Γ t) :=
+⟨inv_image h.r judgment.to_term,
+ inv_image.equivalence h.r judgment.to_term h.iseqv⟩
+
+----
 
 def type.to_string : type → string
 | base := "ι"
@@ -39,267 +169,127 @@ def type.to_string : type → string
 instance : has_to_string type :=
 ⟨type.to_string⟩
 
-def preterm.to_string' : Π {t}, preterm (λ t, ℕ) t → ℕ → string
+def term.to_string' : Π {t}, term (λ t, ℕ) t → ℕ → string
 | _ (var n) _ := to_string n
-| _ (lam f) lv := "(λ" ++ to_string lv ++ "." ++ preterm.to_string' (f lv) (lv + 1) ++ ")"
-| _ (app m₁ m₂) lv := "(" ++ preterm.to_string' m₁ lv ++ " " ++ preterm.to_string' m₂ lv ++ ")"
-| _ (eq m₁ m₂) lv := "(" ++ preterm.to_string' m₁ lv ++ " = " ++ preterm.to_string' m₂ lv ++ ")"
+| _ (lam f) lv := "(λ" ++ to_string lv ++ "." ++ term.to_string' (f lv) (lv + 1) ++ ")"
+| _ (app m₁ m₂) lv := "(" ++ term.to_string' m₁ lv ++ " " ++ term.to_string' m₂ lv ++ ")"
+| _ (eq m₁ m₂) lv := "(" ++ term.to_string' m₁ lv ++ " = " ++ term.to_string' m₂ lv ++ ")"
 
-def preterm.to_string : Preterm t → string :=
-λ m, preterm.to_string' (m _) 0 ++ " : " ++ to_string t
-
-instance : has_to_string (Preterm t) :=
-⟨ preterm.to_string ⟩
-
-def term.to_string' : Π {Γ}, term (λ t, ℕ) Γ t → ℕ → string
-| [] m lv := "⊢ " ++ preterm.to_string' m lv
-| (t :: Γ) f lv := "(" ++ to_string lv ++ " : " ++ to_string t ++ ") " ++ term.to_string' (f lv) (lv + 1)
-
-def term.to_string : Term Γ t → string :=
+def term.to_string : Term t → string :=
 λ m, term.to_string' (m _) 0 ++ " : " ++ to_string t
 
-instance : has_to_string (Term Γ t) :=
-⟨term.to_string⟩
+instance term_has_to_string : has_to_string (Term t) :=
+⟨ term.to_string ⟩
 
-instance : has_repr (Term Γ t) :=
-⟨term.to_string⟩
+def judgment.to_string' : Π {Γ}, judgment (λ t, ℕ) Γ t → ℕ → string
+| [] m lv := "⊢ " ++ term.to_string' m lv
+| (t :: Γ) f lv := "(" ++ to_string lv ++ " : " ++ to_string t ++ ") " ++ judgment.to_string' (f lv) (lv + 1)
 
-----
+def judgment.to_string : Judgment Γ t → string :=
+λ m, judgment.to_string' (m _) 0 ++ " : " ++ to_string t
 
-variables {Γ₁ Γ₂ : list type} {t₁ t₂ t₃ : type}
+instance judgment_has_to_string : has_to_string (Judgment Γ t) :=
+⟨judgment.to_string⟩
 
-def subst' : Π {t : type}, preterm (preterm ν) t → preterm ν t
-| _ (var m) := m
-| _ (lam f) := lam (λ x, subst' (f (var x)))
-| _ (app m₁ m₂) := app (subst' m₁) (subst' m₂)
-| _ (eq m₁ m₂) := eq (subst' m₁) (subst' m₂)
-
-def type.fold : list type → type → type :=
-λ Γ t, list.foldr arrow t Γ
-
-def term.to_preterm' : Π {Γ : list type}, term ν Γ t → preterm ν (type.fold Γ t)
-| [] m := m
-| (t :: Γ) f := lam (λ x, term.to_preterm' (f x))
-
-def term.to_preterm : Term Γ t → Preterm (type.fold Γ t) :=
-λ m ν, term.to_preterm' ν (m ν)
-
-def preterm_subst' : preterm (preterm ν) (arrow t₁ t₂) → preterm ν t₁ → preterm (preterm ν) t₂
-| (lam f) m := f m
-| m₁ m₂ := app m₁ (var m₂)
-
-def preterm.to_term' : Π {Γ : list type}, preterm (preterm ν) (type.fold Γ t) → term ν Γ t
-| [] m := subst' ν m
-| (t :: Γ) m := λ x, preterm.to_term' (preterm_subst' ν m (var x))
-
-def preterm.to_term : Preterm (type.fold Γ t) → Term Γ t :=
-λ m ν, preterm.to_term' ν (m _)
+instance : has_repr (Judgment Γ t) :=
+⟨judgment.to_string⟩
 
 ----
 
-def term.subst' : Π {Γ}, term (preterm ν) (t₁ :: Γ) t₂ → term ν Γ t₁ → term ν Γ t₂
-| [] m₁ m₂ := subst' ν (m₁ m₂)
-| (t :: Γ) f m := λ x, term.subst' (λ x', f x' (var x)) (m x)
+namespace term
+  def top : Term prop :=
+  λ ν, eq (lam (λ x : ν prop, var x)) (lam (λ x, var x))
 
-def term.subst : Term (t₁ :: Γ) t₂ → Term Γ t₁ → Term Γ t₂ :=
-λ m₁ m₂ ν, term.subst' ν (m₁ (preterm ν)) (m₂ ν)
+  def and : Term (arrow prop (arrow prop prop)) :=
+  λ ν, lam (λ p₁, lam (λ p₂, eq (lam (λ f : ν (arrow _ (arrow _ prop)), app (app (var f) (top ν)) (top ν))) (lam (λ f, app (app (var f) (var p₁)) (var p₂)))))
 
-def term.abs' : Π {Γ}, term ν (t₁ :: Γ) t₂ → term ν Γ (arrow t₁ t₂)
-| [] m := lam (λ x, m x)
-| (t :: Γ) f := λ x, term.abs' (λ y, f y x)
+  def Forall : Term (arrow (arrow t prop) prop) :=
+  λ ν, lam (λ f, eq (var f) (lam (λ x, (top ν))))
 
-def term.abs : Term (t₁ :: Γ) t₂ → Term Γ (arrow t₁ t₂) :=
-λ m ν, term.abs' ν (m ν)
+  def bot : Term prop :=
+  λ ν, app (Forall ν) (lam (λ p, var p))
 
-def term.app' : Π {Γ}, term ν Γ (arrow t₁ t₂) → term ν Γ t₁ → term ν Γ t₂
-| [] m₁ m₂ := app m₁ m₂
-| (t :: Γ) f m := λ x, term.app' (f x) (m x)
+  def implies : Term (arrow prop (arrow prop prop)) :=
+  λ ν, lam (λ p₁, lam (λ p₂, eq (app (app (and ν) (var p₁)) (var p₂)) (var p₁)))
 
-def term.app : Term Γ (arrow t₁ t₂) → Term Γ t₁ → Term Γ t₂ :=
-λ m₁ m₂ ν, term.app' ν (m₁ ν) (m₂ ν)
+  def not : Term (arrow prop prop) :=
+  λ ν, lam (λ p, app (app (implies ν) (var p)) (bot ν))
 
-def term.var0' : Π {Γ}, term ν (t :: Γ) t
-| [] := λ x, var x
-| (t :: Γ) := λ x y, term.var0' x
+  def iff : Term (arrow prop (arrow prop prop)):=
+  λ ν, lam (λ p₁, lam (λ p₂, eq (var p₁) (var p₂)))
 
-def term.var0 : Term (t :: Γ) t :=
-λ ν, term.var0' ν
+  def or : Term (arrow prop (arrow prop prop)) :=
+  λ ν, lam (λ p₁, lam (λ p₂, app (Forall ν) (lam (λ r, app (app (implies ν) (app (app (and ν) (app (app (implies ν) (var p₁)) (var r))) (app (app (implies ν) (var p₂)) (var r)))) (var r)))))
 
-def term.weaken1 : Term Γ t₂ → Term (t₁ :: Γ) t₂ :=
-λ m ν x, m ν
+  def Exists : Term (arrow (arrow t prop) prop) :=
+  λ ν, lam (λ f, app (Forall ν) (lam (λ r, app (app (implies ν) (app (Forall ν) (lam (λ x, app (app (implies ν) (app (var f) (var x))) (var r))))) (var r))))
+end term
+open term
 
-def term.weaken : Π {Γ₂ : list type}, Term Γ₁ t → Term (Γ₂ ++ Γ₁) t
-| [] m := m
-| (t :: Γ) m := term.weaken1 (term.weaken m)
-
-def term.var' : Π {Γ}, (t ∈ Γ) → Term Γ t
-| [] h := begin rw list.mem_nil_iff at h, exfalso, assumption end
-| (t' :: Γ) h :=
-  match type.decidable_eq t t' with
-  | (is_true h') := by rw h'; exact term.var0
-  | (is_false h') := term.weaken1 $ term.var' begin
-      rw list.mem_cons_iff at h,
-      cases h with h₁ h₂,
-      { exact absurd h₁ h' },
-      { assumption }
-    end
-  end
-
-def term.var : (t ∈ Γ) → Term Γ t :=
-term.var'
-
-def term.eq' : Π {Γ : list type}, term ν Γ t → term ν Γ t → term ν Γ prop
-| [] m₁ m₂ := eq m₁ m₂
-| (t :: Γ) m₁ m₂ := λ x, term.eq' (m₁ x) (m₂ x)
-
-def term.eq : Term Γ t → Term Γ t → Term Γ prop :=
-λ m₁ m₂ ν, term.eq' ν (m₁ ν) (m₂ ν)
-
------
-
-def domain : type → Type
-| base := preterm ν base
-| prop := preterm ν prop
-| (arrow t₁ t₂) := domain t₁ → domain t₂
-
-def Domain (t : type) : Type 1 :=
-Π ν, domain ν t
-
-def preterm.reify_reflect : Π {t : type}, (domain ν t → preterm ν t) × (preterm ν t → domain ν t)
-| base := ⟨ id, id ⟩
-| prop := ⟨ id, id ⟩
-| (arrow t₁ t₂) :=
-   let r₁ := @preterm.reify_reflect t₁ in
-   let r₂ := @preterm.reify_reflect t₂ in
-   let reify (f : domain ν t₁ → domain ν t₂) := lam (λ x, r₂.1 (f (r₁.2 (var x)))) in
-   let reflect (f : preterm ν (arrow t₁ t₂)) := λ x, r₂.2 (app f (r₁.1 x)) in
-   ⟨reify, reflect⟩
-
-def preterm.reify' : domain ν t → preterm ν t :=
-λ x, (preterm.reify_reflect ν).1 x
-
-def preterm.reify : Domain t → Preterm t :=
-λ m ν, preterm.reify' ν (m _)
-
-def preterm.reflect' : preterm ν t → domain ν t :=
-λ x, (preterm.reify_reflect ν).2 x
-
-def preterm.reflect : Preterm t → Domain t :=
-λ x ν, preterm.reflect' ν (x _)
-
-def preterm.eval' : Π {t : type}, preterm (domain ν) t → (domain ν t)
-| _ (var x) := x
-| _ (lam f) := λ x, preterm.eval' (f x)
-| _ (app m₁ m₂) := (preterm.eval' m₁) (preterm.eval' m₂)
-| _ (eq m₁ m₂) := eq (preterm.reify' ν (preterm.eval' m₁)) (preterm.reify' ν (preterm.eval' m₂))
-
-def preterm.eval : Preterm t → Domain t :=
-λ m ν, preterm.eval' ν (m _)
-
-def preterm.normalize : Preterm t → Preterm t :=
-preterm.reify ∘ preterm.eval
-
-def term.normalize : Term Γ t → Term Γ t :=
-preterm.to_term ∘ preterm.normalize ∘ term.to_preterm
-
-instance : setoid (Term Γ t) :=
-⟨inv_image eq term.normalize,
- inv_image.equivalence eq term.normalize eq.equivalence⟩
-
---------
-
-def weaken : Term [] t → Term Γ t :=
-λ m, by rw ←list.append_nil Γ; from term.weaken m
-
-def term.top : Term Γ prop :=
-weaken $ λ ν, eq (lam (λ x : ν prop, var x)) (lam (λ x, var x))
-
-def term.and : Term Γ (arrow prop (arrow prop prop)) :=
-weaken $ λ ν, lam (λ p₁, lam (λ p₂, eq (lam (λ f : ν (arrow _ (arrow _ prop)), app (app (var f) (@term.top [] ν)) (@term.top [] ν))) (lam (λ f, app (app (var f) (var p₁)) (var p₂)))))
-
-def term.forall : Term Γ (arrow (arrow t prop) prop) :=
-weaken $ λ ν, lam (λ f, eq (var f) (lam (λ x, (@term.top [] ν))))
-
-def term.bot : Term Γ prop :=
-weaken $ λ ν, app (@term.forall [] _ ν) (lam (λ p, var p))
-
-def term.implies : Term Γ (arrow prop (arrow prop prop)) :=
-weaken $ λ ν, lam (λ p₁, lam (λ p₂, eq (app (app (@term.and [] ν) (var p₁)) (var p₂)) (var p₁)))
-
-def term.not : Term Γ (arrow prop prop) :=
-weaken $ λ ν, lam (λ p, app (app (@term.implies [] ν) (var p)) (@term.bot [] ν))
-
-def term.iff : Term Γ (arrow prop (arrow prop prop)):=
-weaken $ λ ν, lam (λ p₁, lam (λ p₂, eq (var p₁) (var p₂)))
-
-def term.or : Term Γ (arrow prop (arrow prop prop)) :=
-weaken $ λ ν, lam (λ p₁, lam (λ p₂, app (@term.forall [] _ ν) (lam (λ r, app (app (@term.implies [] ν) (app (app (@term.and [] ν) (app (app (@term.implies [] ν) (var p₁)) (var r))) (app (app (@term.implies [] ν) (var p₂)) (var r)))) (var r)))))
-
-def term.exists : Term Γ (arrow (arrow t prop) prop) :=
-weaken $ λ ν, lam (λ f, app (@term.forall [] _ ν) (lam (λ r, app (app (@term.implies [] ν) (app (@term.forall [] _ ν) (lam (λ x, app (app (@term.implies [] ν) (app (var f) (var x))) (var r))))) (var r))))
-
-#eval @id (Term [] prop) $ term.app (term.app term.and term.top) (term.app (term.app term.or term.bot) term.top)
+#eval @id (Judgment [] prop) $ app (app and top) (app (app or bot) top)
 
 ----
 
-inductive proof : Π {Γ}, list (Term Γ prop) → Term Γ prop → Prop
-| assump : Π {Γ Φ} {φ : Term Γ prop}, φ ∈ Φ → proof Φ φ
-| refl : Π {Γ Φ t} {m₁ m₂ : Term Γ t}, m₁ ≈ m₂ → proof Φ (term.eq m₁ m₂)
-| cong : Π {Γ Φ t} (m : Term (t :: Γ) prop) (m₂ m₁ : Term Γ t), proof Φ (term.eq m₁ m₂) → proof Φ (term.subst m m₁) → proof Φ (term.subst m m₂)
-| propext : Π {Γ Φ} {φ₁ φ₂ : Term Γ prop}, proof (φ₁ :: Φ) φ₂ → proof (φ₂ :: Φ) φ₁ → proof Φ (term.eq φ₁ φ₂)
-| funext : Π {Γ Φ t₁ t₂} (m₁ m₂ : Term (t₁ :: Γ) t₂), proof (list.map term.weaken1 Φ) (term.eq m₁ m₂) → proof Φ (term.eq (term.abs m₁) (term.abs m₂))
+inductive proof : Π {Γ}, list (Judgment Γ prop) → Judgment Γ prop → Prop
+| assump : Π {Γ Φ} {φ : Judgment Γ prop}, φ ∈ Φ → proof Φ φ
+| refl : Π {Γ Φ t} {m₁ m₂ : Judgment Γ t}, m₁ ≈ m₂ → proof Φ (eq m₁ m₂)
+| cong : Π {Γ Φ t} (m : Judgment (t :: Γ) prop) (m₂ m₁ : Judgment Γ t), proof Φ (eq m₁ m₂) → proof Φ (subst m m₁) → proof Φ (subst m m₂)
+| prop_ext : Π {Γ Φ} {φ₁ φ₂ : Judgment Γ prop}, proof (φ₁ :: Φ) φ₂ → proof (φ₂ :: Φ) φ₁ → proof Φ (eq φ₁ φ₂)
+| fun_ext : Π {Γ Φ t₁ t₂} (m₁ m₂ : Judgment (t₁ :: Γ) t₂), proof (list.map weak Φ) (eq m₁ m₂) → proof Φ (eq (lam m₁) (lam m₂))
 
 -- Let's prove!
 
-example : @proof [prop] [term.var0] (term.eq term.top term.var0) :=
+example : @proof [prop] [var here] (eq (weak top) (var here)) :=
 begin
-  apply proof.propext,
+  apply proof.prop_ext,
   { apply proof.assump,
     simp },
   { apply proof.refl,
     refl }
 end
 
-example : @proof [prop] [term.eq term.top term.var0] term.var0 :=
+example : @proof [prop] [eq (weak top) (var here)] (var here) :=
 begin
-  apply proof.cong (@term.var0 [prop] _) term.var0 term.top,
+  apply proof.cong (var here) (var here) (weak $ @id (Judgment [] prop) top),
   { apply proof.assump,
     simp },
   { apply proof.refl,
     simp }
 end
 
-example {φ₁ φ₂} {Φ : list (Term [] prop)} : @proof [] Φ (term.app (term.app term.and φ₁) φ₂) → @proof [] Φ φ₁ :=
+example {φ₁ φ₂} {Φ : list (Judgment [] prop)} : proof Φ (app (app and φ₁) φ₂) → proof Φ φ₁ :=
 begin
   intro p,
   apply proof.cong
-    term.var0
+    (var here)
     φ₁
     (λ ν, app (lam (λ f, app (app (var f) (φ₁ ν)) (φ₂ ν))) (lam (λ p₁, lam (λ p₂, var p₁)))),
   { apply proof.refl,
     funext,
     refl },
   { apply proof.cong
-      (@id (Term [arrow _ prop] prop) $ λ ν f, app (var f) (lam (λ p₁, lam (λ p₂, var p₁))))
+      (@id (Judgment [arrow _ prop] prop) $ λ ν f, app (var f) (lam (λ p₁, lam (λ p₂, var p₁))))
       (λ ν, lam (λ f, app (app (var f) (φ₁ ν)) (φ₂ ν)))
-      (@id (Term [] (arrow _ prop)) $ λ ν, lam (λ f, app (app (var f) (@term.top [] ν)) (@term.top [] ν))),
+      (@id (Judgment [] (arrow _ prop)) $ λ ν, lam (λ f, app (app (var f) (top ν)) (top ν))),
     { apply proof.cong
-        term.var0
-        (term.eq
-          (@id (Term [] (arrow _ prop)) $ λ ν, lam (λ f, app (app (var f) (@term.top [] ν)) (@term.top [] ν)))
+        (var here)
+        (eq
+          (@id (Judgment [] (arrow _ prop)) $ λ ν, lam (λ f, app (app (var f) (top ν)) (top ν)))
           (λ ν, lam (λ f, app (app (var f) (φ₁ ν)) (φ₂ ν))))
-        (weaken $ λ ν, app (app (lam (λ p₁, lam (λ p₂, eq (lam (λ f : ν (arrow _ (arrow _ prop)), app (app (var f) (@term.top [] ν)) (@term.top [] ν))) (lam (λ f, app (app (var f) (var p₁)) (var p₂)))))) (φ₁ ν)) (φ₂ ν)),
+        (λ ν, app (app (lam (λ p₁, lam (λ p₂, eq (lam (λ f : ν (arrow _ (arrow _ prop)), app (app (var f) (top ν)) (top ν))) (lam (λ f, app (app (var f) (var p₁)) (var p₂)))))) (φ₁ ν)) (φ₂ ν)),
       { apply proof.refl,
         funext,
         refl },
       { from p } },
     { apply proof.cong
-        term.var0
-        (weaken $ (λ ν, app (lam (λ f, app (app (var f) (@term.top [] ν)) (@term.top [] ν))) (lam (λ p₁, lam (λ p₂, var p₁)))))
-        (weaken $ (λ ν, @term.top [] ν) : Term [] prop),
+        (var here)
+        (@id (Judgment [] _) $ λ ν, app (lam (λ f, app (app (var f) (top ν)) (top ν))) (lam (λ p₁, lam (λ p₂, var p₁))))
+        top,
       { apply proof.refl,
         funext,
         refl },
       { apply proof.refl,
         refl } } }
 end
+
+end hol
