src/stlc.lean
@@ -2,7 +2,8 @@
 
 import moromoro
 
-@[derive decidable_eq]
+namespace stlc
+
 inductive type : Type
 | base : type
 | arrow : type → type → type
@@ -12,254 +13,425 @@ def type.to_string : type → string
 | base := "ι"
 | (arrow t₁ t₂) := "(" ++ type.to_string t₁ ++ " → " ++ type.to_string t₂ ++ ")"
 
-instance : has_to_string type :=
+instance type.has_to_string : has_to_string type :=
 ⟨type.to_string⟩
 
 #eval to_string (arrow (arrow base base) base)
 
 ----
 
-variable ν : type → Type
+variables ν : type → Type
 
-inductive preterm : type → Type
-| var : Π {t}, ν t → preterm t
-| lam : Π {t₁ t₂}, (ν t₁ → preterm t₂) → preterm (arrow t₁ t₂)
-| app : Π {t₁ t₂}, preterm (arrow t₁ t₂) → preterm t₁ → preterm t₂
-open preterm
+inductive term : type → Type
+| var : Π {t}, ν t → term t
+| lam : Π {t₁ t₂}, (ν t₁ → term t₂) → term (arrow t₁ t₂)
+| app : Π {t₁ t₂}, term (arrow t₁ t₂) → term t₁ → term t₂
+open term
 
-def Preterm (t : type) : Type 1 :=
-Π ν, preterm ν t
+def Term (t : type) : Type 1 :=
+Π ν, term ν t
 
-def preterm.to_string' : Π {t : type}, preterm (λ t, ℕ) t → ℕ → string
+variables {t t₁ t₂ t₃ : type}
+
+def term.to_string' : Π {t : type}, term (λ t, ℕ) t → ℕ → string
 | _ (var n) _ := to_string n
-| _ (lam f) lv := "(λ" ++ to_string lv ++ "." ++ preterm.to_string' (f lv) (lv + 1) ++ ")"
-| _ (app m₁ m₂) lv := "(" ++ preterm.to_string' m₁ lv ++ " " ++ preterm.to_string' m₂ lv ++ ")"
+| _ (lam f) lv := "(λ" ++ to_string lv ++ "." ++ term.to_string' (f lv) (lv + 1) ++ ")"
+| _ (app m₁ m₂) lv := "(" ++ term.to_string' m₁ lv ++ " " ++ term.to_string' m₂ lv ++ ")"
 
-def preterm.to_string {t : type} : Preterm t → string :=
-λ m, preterm.to_string' (m _) 0 ++ " : " ++ to_string t
+def Term.to_string : Term t → string :=
+λ m, term.to_string' (m _) 0 ++ " : " ++ to_string t
 
-instance {t : type} : has_to_string (Preterm t) :=
-⟨ preterm.to_string ⟩
+instance Term.has_to_string : has_to_string (Term t) :=
+⟨ Term.to_string ⟩
 
-def type.nat := arrow (arrow base base) (arrow base base)
+def nat : type := arrow (arrow base base) (arrow base base)
 
-def zero : Preterm type.nat :=
+def zero : Term nat :=
 λ ν, lam (λ f, lam (λ x, var x))
 
-def succ : Preterm (arrow type.nat type.nat) :=
+def succ : Term (arrow nat nat) :=
 λ ν, lam (λ n, lam (λ f, lam (λ x, app (var f) (app (app (var n) (var f)) (var x)))))
 
-def succ_zero : Preterm type.nat :=
-(λ ν, app (succ ν) (zero ν))
+def App : Term (arrow t₁ t₂) → Term t₁ → Term t₂ :=
+λ m₁ m₂ ν, app (m₁ ν) (m₂ ν)
+
+def succ_zero : Term nat :=
+App succ zero
 
 #eval to_string zero      -- "(λ0.(λ1.1)) : ((ι → ι) → (ι → ι))"
 #eval to_string succ      -- "(λ0.(λ1.(λ2.(1 ((0 1) 2))))) : (((ι → ι) → (ι → ι)) → ((ι → ι) → (ι → ι)))"
 #eval to_string succ_zero -- "((λ0.(λ1.(λ2.(1 ((0 1) 2))))) (λ0.(λ1.1))) : ((ι → ι) → (ι → ι))"
 
--- // error!
--- def ω : Preterm _ := -- no such type
+-- -- // error!
+-- def ω : Term _ := -- no such type
 -- λ ν, lam (λ x, app (var x) (var x))
 
 ----
 
--- def term0 (t : type) := Π ν, preterm ν t
--- def term1 (t₁ t₂ : type) := Π ν, ν t₁ → preterm ν t₂ -- preterm with one free variable
+def domain : type → Type
+| base := term ν base
+| (arrow t₁ t₂) := domain t₁ → domain t₂
 
--- inductive term : list type → type → Type
--- | empty : Π {t}, preterm ν t → term [] t
--- | extend : Π {t₁ t₂ Γ}, (ν t₁ → term Γ t₂) → term (t₁ :: Γ) t₂
+def Domain (t : type) : Type 1 :=
+Π ν, domain ν t
 
-def term : list type → type → Type :=
-λ Γ t, list.foldr (λ t α, ν t → α) (preterm ν t) Γ
+-- def nbe_wf : psum (Σ' {t : type}, domain ν t) (Σ' {t : type}, term ν t) → ℕ :=
+-- λ v, match v with
+-- | (psum.inl x) := sizeof x.fst
+-- | (psum.inr x) := sizeof x.fst
+-- end
 
-def Term (Γ : list type) (t : type) : Type 1 := -- Type 1
-Π ν, term ν Γ t
+-- mutual def reify, reflect
+-- with reify : Π {t : type}, domain ν t → term ν t
+-- | base ν := ν
+-- | (arrow t₁ t₂) f := lam (λ x, reify (f (reflect (var x))))
+-- with reflect : Π {t : type}, term ν t → domain ν t
+-- | base m := m
+-- | (arrow t₁ t₂) f := λ x, reflect (app f (reify x))
+-- using_well_founded
+-- { rel_tac := λ _ _, `[exact ⟨_, measure_wf (nbe_wf ν)⟩] }
 
-#reduce Term [] base           -- Π ν, preterm ν base
-#reduce Term [base] base       -- Π ν, ν base → preterm ν base
-#reduce Term [base, base] base -- Π ν, ν base → ν base → preterm ν base
+def reify_reflect : Π (t : type), (domain ν t → term ν t) × (term ν t → domain ν t)
+| base := ⟨ id, id ⟩
+| (arrow t₁ t₂) :=
+   let r₁ := reify_reflect t₁ in
+   let r₂ := reify_reflect t₂ in
+   let reify (f : domain ν t₁ → domain ν t₂) := lam (λ x, r₂.1 (f (r₁.2 (var x)))) in
+   let reflect (f : term ν (arrow t₁ t₂)) := λ x, r₂.2 (app f (r₁.1 x)) in
+   ⟨reify, reflect⟩
 
-variables {Γ : list type} {t : type}
+def reify : Domain t → Term t :=
+λ x ν, (reify_reflect ν t).1 (x ν)
 
-def term.to_string' : Π {Γ : list type}, term (λ t, ℕ) Γ t → ℕ → string
-| [] m lv := "⊢ " ++ preterm.to_string' m lv
-| (t :: Γ) f lv := "(" ++ to_string lv ++ " : " ++ to_string t ++ ") " ++ term.to_string' (f lv) (lv + 1)
+def eval' : Π {t : type}, term (domain ν) t → domain ν t
+| _ (var x) := x
+| _ (lam f) := λ x, eval' (f x)
+| _ (app m₁ m₂) := (eval' m₁) (eval' m₂)
 
-def term.to_string : Term Γ t → string :=
-λ m, term.to_string' (m _) 0 ++ " : " ++ to_string t
+def eval : Term t → Domain t :=
+λ m ν, eval' ν (m _)
 
-instance : has_to_string (Term Γ t) :=
-⟨term.to_string⟩
+def normalize : Term t → Term t :=
+reify ∘ eval
 
-def ex1 : Term [arrow base base, base] (arrow base base) :=
-λ ν, λ x₁ x₂, lam (λ y, var x₂)
+#eval to_string $ normalize zero
+#eval to_string $ normalize (App succ zero)
+#eval to_string $ normalize (App succ (App succ zero))
+#eval to_string $ normalize (App succ (App succ (App succ zero)))
 
-#eval to_string ex1 -- "(0 : (ι → ι)) (1 : ι) ⊢ (λ2.1) : (ι → ι)"
+def i : Term (arrow (arrow base base) (arrow base base)) :=
+λ ν, lam (λ f, var f)
+
+#eval to_string i
+#eval to_string $ normalize i
+
+instance : setoid (Term t) :=
+⟨inv_image eq normalize,
+ inv_image.equivalence eq normalize eq.equivalence⟩
+
+def one : Term (arrow (arrow base base) (arrow base base)) :=
+λ ν, lam (λ f, lam (λ x, app (var f) (var x)))
+
+lemma zero_approx_zero : zero ≈ zero :=
+by reflexivity
+
+lemma succ_zero_approx_one : App succ zero ≈ one :=
+begin
+  unfold has_equiv.equiv setoid.r inv_image,
+  reflexivity
+end
+
+----
+
+variable {α : Type}
+
+inductive mem : α → list α → Type
+| here : Π {x l}, mem x (x :: l)
+| there : Π {x l y}, mem x l → mem x (y :: l)
+open mem
+
+local infix ` ∈ ` := mem
+
+inductive judgment₁ : list type → type → Type
+| var : Π {Γ t}, t ∈ Γ → judgment₁ Γ t
+| lam : Π {Γ t₁ t₂}, judgment₁ (t₁ :: Γ) t₂ → judgment₁ Γ (arrow t₁ t₂)
+| app : Π {Γ t₁ t₂}, judgment₁ Γ (arrow t₁ t₂) → judgment₁ Γ t₁ → judgment₁ Γ t₂
+open judgment₁
+
+variables {Γ Γ₁ Γ₂ : list type}
+
+def judgment₁.to_string' : Π {Γ t}, judgment₁ Γ t → string
+| Γ _ (var h) := to_string $ Γ.length - 1 - (h.rec_on (λ _ _, 0) (λ _ _ _ _ (n : ℕ), n + 1))
+| Γ _ (lam m) := "(λ" ++ to_string Γ.length ++ "." ++ judgment₁.to_string' m ++ ")"
+| _ _ (app m₁ m₂) := "(" ++ judgment₁.to_string' m₁ ++ " " ++ judgment₁.to_string' m₂ ++ ")"
+
+def judgment₁.to_string : Π {Γ t}, judgment₁ Γ t → string :=
+λ Γ t m,
+let env := (Γ.foldr (λ t p, prod.mk (prod.mk p.2 t :: p.1) (p.2 + 1)) (prod.mk [] 0)).1 in
+let assigns := list.map (λ p, to_string (prod.fst p) ++ " : " ++ to_string (prod.snd p)) env in
+string.intercalate ", " assigns ++ " ⊢ " ++ judgment₁.to_string' m ++ " : " ++ to_string t
+
+instance : has_to_string (judgment₁ Γ t) :=
+⟨judgment₁.to_string⟩
+
+-- x₁ : ι → ι, x₀ : ι ⊢ λ y, x₀ : (ι → ι) → ι
+def ex1 : judgment₁ [arrow base base, base] (arrow (arrow base base) base) :=
+lam (var (there (there here)))
+
+#eval to_string ex1 -- "1 : (ι → ι), 0 : ι ⊢ (λ2.0) : ((ι → ι) → ι)"
+
+----
+
+inductive perm : list α → list α → Type -- proof relevant version
+| nil   : perm [] []
+| skip  : Π {x : α} {l₁ l₂ : list α}, perm l₁ l₂ → perm (x :: l₁) (x :: l₂)
+| swap  : Π {x y : α} {l : list α}, perm (y :: x :: l) (x :: y :: l)
+| trans : Π {l₁ l₂ l₃ : list α}, perm l₁ l₂ → perm l₂ l₃ → perm l₁ l₃
+
+local infix ~ := perm
+
+def mem_perm {t : α} : Π {Γ₁ Γ₂}, Γ₁ ~ Γ₂ → t ∈ Γ₁ → t ∈ Γ₂
+| _ _ perm.nil h := h
+| _ _ (perm.skip _) here := here
+| _ _ (perm.skip p) (there h) := there (mem_perm p h)
+| _ _ perm.swap here := there here
+| _ _ perm.swap (there here) := here
+| _ _ perm.swap (there (there h)) := there (there h)
+| _ _ (perm.trans p₁ p₂) h := mem_perm p₂ (mem_perm p₁ h)
+
+namespace judgment₁
+
+def xchg : Π {Γ₁ Γ₂ t}, (Γ₁ ~ Γ₂) → judgment₁ Γ₁ t → judgment₁ Γ₂ t
+| _ _ _ p (var h) := var (mem_perm p h)
+| _ _ _ p (lam m) := lam (xchg (perm.skip p) m)
+| _ _ _ p (app m₁ m₂) := app (xchg p m₁) (xchg p m₂)
+
+def weak : Π {Γ t₁ t₂}, judgment₁ Γ t₁ → judgment₁ (t₂ :: Γ) t₁
+| _ _ _ (var h) := var (there h)
+| _ _ _ (lam m) := lam (xchg perm.swap (weak m))
+| _ _ _ (app m₁ m₂) := app (weak m₁) (weak m₂)
+
+def heightof : Π {Γ t}, judgment₁ Γ t → ℕ
+| _ _ (var h) := 1
+| _ _ (lam m) := 1 + heightof m
+| _ _ (app m₁ m₂) := 1 + max (heightof m₁) (heightof m₂)
+
+lemma height_xchg_eq_height {m : judgment₁ Γ₁ t} : Π {Γ₂} {p : Γ₁ ~ Γ₂}, heightof (xchg p m) = heightof m :=
+begin
+  induction m with _ _ _ _ _ _ _ ih₁ _ _ _ _ _ ih₂ ih₃,
+  { intros, refl },
+  { intros, unfold xchg heightof, rw ih₁ },
+  { intros, unfold xchg heightof, rw [ih₂, ih₃] }
+end
+
+def subst : Π {Γ t₁ t₂}, judgment₁ (t₁ :: Γ) t₂ → judgment₁ Γ t₁ → judgment₁ Γ t₂
+| _ _ _ (var here) m := m
+| _ _ _ (var (there h)) m := var h
+| _ _ _ (app m₁ m₂) m :=
+  have heightof m₁ < heightof (app m₁ m₂),
+    by unfold heightof; rw add_comm;
+    from lt_add_of_le_of_pos (le_max_left _ _) zero_lt_one,
+  have heightof m₂ < heightof (app m₁ m₂),
+    by unfold heightof; rw add_comm;
+    from lt_add_of_le_of_pos (le_max_right _ _) zero_lt_one,
+  app (subst m₁ m) (subst m₂ m)
+| _ _ _ (lam m₁) m :=
+  have heightof (xchg perm.swap m₁) < heightof (lam m₁),
+    by unfold heightof; rw height_xchg_eq_height;
+    from lt_add_of_pos_of_le zero_lt_one (le_refl _),
+  lam (subst (xchg perm.swap m₁) (weak m))
+using_well_founded
+{ rel_tac := λ _ _, `[exact ⟨_, measure_wf (λ v, heightof v.snd.snd.snd.fst)⟩] }
+
+def contr : judgment₁ (t₁ :: t₁ :: Γ) t₂ → judgment₁ (t₁ :: Γ) t₂ :=
+λ m, subst m (var here)
 
 ---- 
 
-variables {t₁ t₂ : type}
+inductive env : list type → Type
+| nil {} : env []
+| step : Π {t Γ}, ν t → env Γ →  env (t :: Γ)
 
-def subst' : Π {t : type}, preterm (preterm ν) t → preterm ν t
-| _ (var m) := m
-| _ (lam f) := lam (λ x, subst' (f (var x)))
-| _ (app m₁ m₂) := app (subst' m₁) (subst' m₂)
+def to_term_var : Π {Γ t}, t ∈ Γ → env ν Γ → term ν t
+| (_ :: Γ) _ here (env.step x _) := term.var x
+| (_ :: Γ) _ (there h) (env.step _ Δ) := to_term_var h Δ
+
+def to_term' : Π {Γ t}, judgment₁ Γ t → env ν Γ → term ν t
+| _ _ (var h) Δ := to_term_var ν h Δ
+| _ _ (lam m) Δ := term.lam (λ x, to_term' m (env.step x Δ))
+| _ _ (app m₁ m₂) Δ := term.app (to_term' m₁ Δ) (to_term' m₂ Δ)
+
+def type.foldl : list type → type → type :=
+λ Γ t, list.foldl (λ r t, arrow t r) t Γ
+
+#eval _root_.to_string $ type.foldl [arrow base base, base] base -- "(ι → ((ι → ι) → ι))"
+
+def foldl : Π {Γ t}, judgment₁ Γ t → judgment₁ [] (type.foldl Γ t)
+| [] _ m := m
+| (t :: Γ) _ m := foldl (lam m)
+
+def to_term : judgment₁ Γ t → Term (type.foldl Γ t) :=
+λ m ν, to_term' ν (foldl m) env.nil
+
+end judgment₁
+
+----
+
+variables {ν₁ ν₂ : type → Type}
+
+inductive wf : list (Σ t, ν₁ t × ν₂ t) → Π {t}, term ν₁ t → term ν₂ t → Type
+| var : Π {Γ t} {x₁ : ν₁ t} {x₂ : ν₂ t}, sigma.mk t (prod.mk x₁ x₂) ∈ Γ → wf Γ (var x₁) (var x₂)
+| lam : Π {Γ t₁ t₂} {f₁ : ν₁ t₁ → term ν₁ t₂} {f₂ : ν₂ t₁ → term ν₂ t₂}, (Π x₁ x₂, wf (⟨t₁, x₁, x₂⟩ :: Γ) (f₁ x₁) (f₂ x₂)) → wf Γ (lam f₁) (lam f₂)
+| app : Π {Γ t₁ t₂} {m₁ : term ν₁ (arrow t₁ t₂)} {m₂ : term ν₂ (arrow t₁ t₂)} {n₁ : term ν₁ t₁} {n₂ : term ν₂ t₁}, wf Γ m₁ m₂ → wf Γ n₁ n₂ → wf Γ (app m₁ n₁) (app m₂ n₂)
+
+def WF (t : type) (m : Term t) : Type 1 :=
+Π ν₁ ν₂, wf [] (m ν₁) (m ν₂)
+
+constant term_wf : Π t m, WF t m
+
+def to_judgment₁_var : Π {Γ t} {x₁ : ν₁ t} {x₂ : ν₂ t}, (sigma.mk t (prod.mk x₁ x₂)) ∈ Γ → t ∈ (list.map (λ x, sigma.fst x) Γ)
+| _ _ _ _ here := here
+| _ _ _ _ (there h) := there (to_judgment₁_var h)
+
+def to_judgment₁' : Π {Γ t} {m₁ : term (λ x, unit) t} {m₂ : term (λ x, unit) t}, wf Γ m₁ m₂ → judgment₁ (list.map (λ x, sigma.fst x) Γ) t
+| _ _ _ _ (wf.var h) := var (to_judgment₁_var h)
+| _ _ _ _ (wf.lam f) := lam (to_judgment₁' (f () ()))
+| _ _ _ _ (wf.app m₁ m₂) := app (to_judgment₁' m₁) (to_judgment₁' m₂)
+
+noncomputable def to_judgment₁ : Term t → judgment₁ [] t := 
+λ m, to_judgment₁' (term_wf _ m _ _)
+
+--------------
+
+-- def judgment0 (t : type) := Π ν, term ν t
+-- def judgment1 (t₁ t₂ : type) := Π ν, ν t₁ → term ν t₂ -- term with one free variable
+
+-- inductive judgment₂ : list type → type → Type
+-- | empty : Π {t}, term ν t → judgment₂ [] t
+-- | extend : Π {t₁ t₂ Γ}, (ν t₁ → judgment₂ Γ t₂) → judgment₂ (t₁ :: Γ) t₂
+
+def judgment₂ : list type → type → Type :=
+λ Γ t, list.foldr (λ t α, ν t → α) (term ν t) Γ
+
+def Judgment₂ (Γ : list type) (t : type) : Type 1 := -- Type 1
+Π ν, judgment₂ ν Γ t
+
+#reduce Judgment₂ [] base           -- Π ν, term ν base
+#reduce Judgment₂ [base] base       -- Π ν, ν base → term ν base
+#reduce Judgment₂ [base, base] base -- Π ν, ν base → ν base → term ν base
+
+def judgment₂.to_string' : Π {Γ}, judgment₂ (λ t, ℕ) Γ t → ℕ → string
+| [] m lv := "⊢ " ++ term.to_string' m lv
+| (t :: Γ) f lv := "(" ++ to_string lv ++ " : " ++ to_string t ++ ") " ++ judgment₂.to_string' (f lv) (lv + 1)
+
+def judgment₂.to_string : Judgment₂ Γ t → string :=
+λ m, judgment₂.to_string' (m _) 0 ++ " : " ++ to_string t
+
+instance Judgment₂_has_to_string : has_to_string (Judgment₂ Γ t) :=
+⟨judgment₂.to_string⟩
+
+def ex2 : Judgment₂ [arrow base base, base] (arrow base base) :=
+λ ν, λ x₁ x₂, lam (λ y, var x₂)
+
+#eval to_string ex2 -- "(0 : (ι → ι)) (1 : ι) ⊢ (λ2.1) : (ι → ι)"
+
+---- 
 
 def type.fold : list type → type → type :=
 λ Γ t, list.foldr arrow t Γ
 
-def term.to_preterm' : Π {Γ : list type}, term ν Γ t → preterm ν (type.fold Γ t)
+namespace judgment₂
+def to_term' : Π {Γ}, judgment₂ ν Γ t → term ν (type.fold Γ t)
 | [] m := m
-| (t :: Γ) f := lam (λ x, term.to_preterm' (f x))
+| (t :: Γ) f := lam (λ x, to_term' (f x))
 
-def term.to_preterm : Term Γ t → Preterm (type.fold Γ t) :=
-λ m ν, term.to_preterm' ν (m ν)
+def to_term : Judgment₂ Γ t → Term (type.fold Γ t) :=
+λ m ν, to_term' ν (m ν)
+end judgment₂
 
-def preterm_subst' : preterm (preterm ν) (arrow t₁ t₂) → preterm ν t₁ → preterm (preterm ν) t₂
+def subst' : Π {t}, term (term ν) t → term ν t
+| _ (var m) := m
+| _ (lam f) := lam (λ x, subst' (f (var x)))
+| _ (app m₁ m₂) := app (subst' m₁) (subst' m₂)
+
+def subst'' : term (term ν) (arrow t₁ t₂) → term ν t₁ → term (term ν) t₂
 | (lam f) m := f m
 | m₁ m₂ := app m₁ (var m₂)
 
-def preterm.to_term' : Π {Γ : list type}, preterm (preterm ν) (type.fold Γ t) → term ν Γ t
+def to_judgment₂' : Π {Γ}, term (term ν) (type.fold Γ t) → judgment₂ ν Γ t
 | [] m := subst' ν m
-| (t :: Γ) m := λ x, preterm.to_term' (preterm_subst' ν m (var x))
+| (t :: Γ) m := λ x, to_judgment₂' (subst'' ν m (var x))
 
-def preterm.to_term : Preterm (type.fold Γ t) → Term Γ t :=
-λ m ν, preterm.to_term' ν (m _)
+def to_judgment₂ : Term (type.fold Γ t) → Judgment₂ Γ t :=
+λ m ν, to_judgment₂' ν (m _)
 
 -----
 
-variables {Γ₁ Γ₂ : list type}
+namespace judgment₂
 
-def term.subst' : Π {Γ}, term (preterm ν) (t₁ :: Γ) t₂ → term ν Γ t₁ → term ν Γ t₂
-| [] m₁ m₂ := subst' ν (m₁ m₂)
-| (t :: Γ) f m := λ x, term.subst' (λ x', f x' (var x)) (m x)
-
-def term.subst : Term (t₁ :: Γ) t₂ → Term Γ t₁ → Term Γ t₂ :=
-λ m₁ m₂ ν, term.subst' ν (m₁ (preterm ν)) (m₂ ν)
-
-def term.abs' : Π {Γ}, term ν (t₁ :: Γ) t₂ → term ν Γ (arrow t₁ t₂)
-| [] m := lam (λ x, m x)
-| (t :: Γ) f := λ x, term.abs' (λ y, f y x)
-
-def term.abs : Term (t₁ :: Γ) t₂ → Term Γ (arrow t₁ t₂) :=
-λ m ν, term.abs' ν (m ν)
-
-def term.app' : Π {Γ}, term ν Γ (arrow t₁ t₂) → term ν Γ t₁ → term ν Γ t₂
-| [] m₁ m₂ := app m₁ m₂
-| (t :: Γ) f m := λ x, term.app' (f x) (m x)
-
-def term.app : Term Γ (arrow t₁ t₂) → Term Γ t₁ → Term Γ t₂ :=
-λ m₁ m₂ ν, term.app' ν (m₁ ν) (m₂ ν)
-
-def term.var0' : Π {Γ}, term ν (t :: Γ) t
-| [] := λ x, var x
-| (t :: Γ) := λ x y, term.var0' x
-
-def term.var0 : Term (t :: Γ) t :=
-λ ν, term.var0' ν
-
-def term.contr : Term (t₁ :: t₁ :: Γ) t₂ → Term (t₁ :: Γ) t₂ :=
-λ m, term.subst m term.var0 -- corollary
-
-def term.weaken1 : Term Γ t₂ → Term (t₁ :: Γ) t₂ :=
+def weak : Judgment₂ Γ t₂ → Judgment₂ (t₁ :: Γ) t₂ :=
 λ m ν x, m ν
 
-def term.weaken' : Π {Γ₂ : list type}, Term Γ₁ t → Term (Γ₂ ++ Γ₁) t
-| [] m := m
-| (t :: Γ) m := term.weaken1 (term.weaken' m)
-
-def term.weaken : Term Γ₁ t → Term (Γ₂ ++ Γ₁) t :=
-term.weaken'
-
-def term.var₁ : Term (Γ₁ ++ t ::  Γ₂) t :=
-term.weaken term.var0
-
-inductive perm {α : Type} : list α → list α → Type -- proof relevant version
-| nil   : perm [] []
-| skip  : Π (x : α) {l₁ l₂ : list α}, perm l₁ l₂ → perm (x :: l₁) (x :: l₂)
-| swap  : Π (x y : α) (l : list α), perm (y :: x :: l) (x :: y :: l)
-| trans : Π {l₁ l₂ l₃ : list α}, perm l₁ l₂ → perm l₂ l₃ → perm l₁ l₃
-
-infix ~ := perm
-
-def term.exchange' : Π {Γ₁ Γ₂ : list type}, (Γ₁ ~ Γ₂) → term ν Γ₁ t → term ν Γ₂ t
+def xchg' : Π {Γ₁ Γ₂}, (Γ₁ ~ Γ₂) → judgment₂ ν Γ₁ t → judgment₂ ν Γ₂ t
 | _ _ perm.nil m := m
-| _ _ (perm.skip _ h) m := λ x, term.exchange' h (m x)
-| _ _ (perm.swap _ _ _) m := λ x₁ x₂, m x₂ x₁
-| _ _ (perm.trans h₁ h₂) m := term.exchange' h₂ (term.exchange' h₁ m)
+| _ _ (perm.skip h) m := λ x, xchg' h (m x)
+| _ _ perm.swap m := λ x₁ x₂, m x₂ x₁
+| _ _ (perm.trans h₁ h₂) m := xchg' h₂ (xchg' h₁ m)
 
-def term.exchange : (Γ₁ ~ Γ₂) → Term Γ₁ t → Term Γ₂ t :=
-λ h m ν, term.exchange' ν h (m ν)
+def xchg : (Γ₁ ~ Γ₂) → Judgment₂ Γ₁ t → Judgment₂ Γ₂ t :=
+λ h m ν, xchg' ν h (m ν)
 
-def term.var₂ : (t :: Γ₁ ~ Γ₂) → Term Γ₂ t :=
-λ h, term.exchange h term.var0
+def subst''' : Π {Γ}, judgment₂ (term ν) (t₁ :: Γ) t₂ → judgment₂ ν Γ t₁ → judgment₂ ν Γ t₂
+| [] m₁ m₂ := subst' ν (m₁ m₂)
+| (t :: Γ) f m := λ x, subst''' (λ x', f x' (var x)) (m x)
 
--- def type.has_dec_eq : decidable_eq type
--- | base base := is_true rfl
--- | (arrow t₁ t₂) base := is_false (λ h, type.no_confusion h)
--- | base (arrow t₁ t₂) := is_false (λ h, type.no_confusion h)
--- | (arrow t₁ t₂) (arrow s₁ s₂) :=
---   match type.has_dec_eq t₁ s₁ with
---   | (is_true h) :=
---     match type.has_dec_eq t₂ s₂ with
---     | (is_true h') := is_true (h' ▸ h ▸ rfl)
---     | (is_false h') := is_false (λ h'', type.no_confusion h'' (λ h₁ h₂, absurd h₂ h'))
---     end
---   | (is_false h) := is_false (λ h', type.no_confusion h' (λ h₁ h₂, absurd h₁ h))
---   end
+def subst : Judgment₂ (t₁ :: Γ) t₂ → Judgment₂ Γ t₁ → Judgment₂ Γ t₂ :=
+λ m₁ m₂ ν, subst''' ν (m₁ _) (m₂ ν)
 
--- instance type_dec_eq : decidable_eq type :=
--- --type.has_dec_eq
--- by tactic.mk_dec_eq_instance
+def lam' : Π {Γ}, judgment₂ ν (t₁ :: Γ) t₂ → judgment₂ ν Γ (arrow t₁ t₂)
+| [] m := lam (λ x, m x)
+| (t :: Γ) f := λ x, lam' (λ y, f y x)
 
-def term.var' : Π {Γ}, (t ∈ Γ) → Term Γ t
-| [] h := begin rw list.mem_nil_iff at h, exfalso, assumption end
-| (t' :: ts) h :=
-  match type.decidable_eq t t' with
-  | (is_true h') := by rw h'; exact term.var0
-  | (is_false h') := term.weaken1 $ @term.var' ts begin
-      rw list.mem_cons_iff at h,
-      cases h with h₁ h₂,
-      { exact absurd h₁ h' },
-      { assumption }
-    end
-  end
+def lam : Judgment₂ (t₁ :: Γ) t₂ → Judgment₂ Γ (arrow t₁ t₂) :=
+λ m ν, lam' ν (m ν)
 
-def term.var : (t ∈ Γ) → Term Γ t :=
-term.var'
+def app' : Π {Γ}, judgment₂ ν Γ (arrow t₁ t₂) → judgment₂ ν Γ t₁ → judgment₂ ν Γ t₂
+| [] m₁ m₂ := app m₁ m₂
+| (t :: Γ) f m := λ x, app' (f x) (m x)
 
-def term.nonfree₁' : Π {t : type}, preterm (λ t, Prop) t → Prop
-| _ (var x) := x
-| _ (lam f) := term.nonfree₁' (f true)
-| _ (app m₁ m₂) := term.nonfree₁' m₁ ∧ term.nonfree₁' m₂
+def app : Judgment₂ Γ (arrow t₁ t₂) → Judgment₂ Γ t₁ → Judgment₂ Γ t₂ :=
+λ m₁ m₂ ν, app' ν (m₁ ν) (m₂ ν)
 
-def term.nonfree₁'' : Π {Γ : list type}, term (λ t, Prop) (t₁ :: Γ) t₂ → Prop
-| [] m := term.nonfree₁' (m false)
-| (t :: Γ) m := term.nonfree₁'' (λ x, m x true)
+def var' : Π {Γ}, judgment₂ ν (t :: Γ) t
+| [] := λ x, var x
+| (t :: Γ) := λ x y, var' x
 
-def term.nonfree₁ : Term (t₁ :: Γ) t₂ → Prop :=
-λ m, term.nonfree₁'' (m _)
+def var : Π {Γ}, t ∈ Γ → Judgment₂ Γ t
+| _ here := λ ν, var' ν
+| _ (there h) := weak (var h)
 
--- def term.free' : Π {t : type}, preterm (λ t, Prop) t → Prop
--- | _ (var x) := x
--- | _ (lam f) := term.free' (f true)
--- | _ (app m₁ m₂) := term.free' m₁ ∧ term.free' m₂
--- | _ (id m₁ m₂) := term.free' m₁ ∧ term.free' m₂
+def contr : Judgment₂ (t₁ :: t₁ :: Γ) t₂ → Judgment₂ (t₁ :: Γ) t₂ := -- same as judgment₁.contr
+λ m, subst m (var here)
 
--- def term.free'' : Π {Γ : list type}, term (λ t, Prop) (t₁ :: Γ) t₂ → Prop
--- | [] m := term.free' (m false)
--- | (t :: Γ) m := term.free'' (λ x, m x true)
+def nonfree₁' : Π {t : type}, term (λ t, Prop) t → Prop
+| _ (term.var x) := x
+| _ (term.lam f) := nonfree₁' (f true)
+| _ (term.app m₁ m₂) := nonfree₁' m₁ ∧ nonfree₁' m₂
 
--- def term.free : Term (t₁ :: Γ) t₂ → Prop :=
--- λ m, term.free'' (m _)
+def nonfree₁'' : Π {Γ : list type}, judgment₂ (λ t, Prop) (t₁ :: Γ) t₂ → Prop
+| [] m := nonfree₁' (m false)
+| (t :: Γ) m := nonfree₁'' (λ x, m x true)
 
-def term.nonfree₂ (m : Term (t₁ :: Γ) t₂) : Prop :=
-∃ m', m = term.weaken1 m'
+def nonfree₁ : Judgment₂ (t₁ :: Γ) t₂ → Prop :=
+λ m, nonfree₁'' (m _)
 
-lemma nonfree_var_lem (m : Term (t₁ :: Γ) t₂)
-: term.nonfree₂ m ↔ ∃ (m' : Term Γ t₂), ∀ ν, (λ x, (m ν) x) = (λ x, (m' ν)) :=
+def nonfree₂ (m : Judgment₂ (t₁ :: Γ) t₂) : Prop :=
+∃ m', m = weak m'
+
+lemma nonfree_var_lem (m : Judgment₂ (t₁ :: Γ) t₂)
+: nonfree₂ m ↔ ∃ (m' : Judgment₂ Γ t₂), ∀ ν, (λ x, (m ν) x) = (λ x, (m' ν)) :=
 begin
-  unfold term.nonfree₂,
+  unfold nonfree₂,
   split,
   { intro h,
     induction h,
@@ -273,84 +445,28 @@ begin
     apply funext h_h }
 end
 
-def term.nonfree (m : Term (t₁ :: Γ) t₂) := -- proof relevant version
-{ m' : Term Γ t₂ // m = term.weaken1 m' }
+end judgment₂
 
-----
+-- instance : setoid (Judgment₂ Γ t) :=
+-- ⟨inv_image eq (normalize ∘ judgment₂.to_term),
+--  inv_image.equivalence eq (normalize ∘ judgment₂.to_term) eq.equivalence⟩
 
-def domain : type → Type
-| base := preterm ν base
-| (arrow t₁ t₂) := domain t₁ → domain t₂
+-- def zero' : Judgment₂ [] (arrow (arrow base base) (arrow base base)) :=
+-- to_judgment₂ zero
 
-def Domain (t : type) : Type 1 :=
-Π ν, domain ν t
+-- def one' : Judgment₂ [] (arrow (arrow base base) (arrow base base)) :=
+-- to_judgment₂ one
 
--- mutual def reify', reflect'
--- with reify' : Π {t : type}, domain ν t → preterm ν t
--- | base ν := v
--- | (arrow t₁ t₂) f := lam (λ x, reify' (f (reflect' (var x))))
--- with reflect' : Π {t : type}, preterm ν t → domain ν t
--- | base m := m
--- | (arrow t₁ t₂) f := λ x, reflect' (app f (reify' x))
+-- def succ' : Judgment₂ [] (arrow (arrow (arrow base base) (arrow base base)) (arrow (arrow base base) (arrow base base))) :=
+-- to_judgment₂ succ
 
-def preterm.reify_reflect : Π {t : type}, (domain ν t → preterm ν t) × (preterm ν t → domain ν t)
-| base := ⟨ id, id ⟩
-| (arrow t₁ t₂) :=
-   let r₁ := @preterm.reify_reflect t₁ in
-   let r₂ := @preterm.reify_reflect t₂ in
-   let reify (f : domain ν t₁ → domain ν t₂) := lam (λ x, r₂.1 (f (r₁.2 (var x)))) in
-   let reflect (f : preterm ν (arrow t₁ t₂)) := λ x, r₂.2 (app f (r₁.1 x)) in
-   ⟨reify, reflect⟩
+-- lemma zero_approx_zero : zero' ≈ zero' :=
+-- by reflexivity
 
-def preterm.reify : Domain t → Preterm t :=
-λ x ν, (preterm.reify_reflect ν).1 (x ν)
+-- lemma succ_zero_approx_one : judgment₂.app succ' zero' ≈ one' :=
+-- begin
+--   unfold has_equiv.equiv setoid.r inv_image,
+--   reflexivity
+-- end
 
-def preterm.reflect : Preterm t → Domain t :=
-λ x ν, (preterm.reify_reflect ν).2 (x ν)
-
-def preterm.eval' : Π {t : type}, preterm (domain ν) t → (domain ν t)
-| _ (var x) := x
-| _ (lam f) := λ x, preterm.eval' (f x)
-| _ (app m₁ m₂) := (preterm.eval' m₁) (preterm.eval' m₂)
-
-def preterm.eval : Preterm t → Domain t :=
-λ m ν, preterm.eval' ν (m _)
-
-def preterm.normalize : Preterm t → Preterm t :=
-preterm.reify ∘ preterm.eval
-
-def term.normalize : Term Γ t → Term Γ t :=
-preterm.to_term ∘ preterm.normalize ∘ term.to_preterm
-
-def term.zero : Term [] (arrow (arrow base base) (arrow base base)) :=
-λ ν, lam (λ f, lam (λ x, var x))
-
-def term.succ : Term [] (arrow (arrow (arrow base base) (arrow base base)) (arrow (arrow base base) (arrow base base))) :=
-λ ν, lam (λ n, lam (λ f, lam (λ x, app (var f) (app (app (var n) (var f)) (var x)))))
-
-#eval to_string $ term.normalize term.zero
-#eval to_string $ term.normalize (term.app term.succ zero)
-#eval to_string $ term.normalize (term.app term.succ (term.app term.succ term.zero))
-#eval to_string $ term.normalize (term.app term.succ (term.app term.succ (term.app term.succ term.zero)))
-
-def i_nat : Term [] (arrow (arrow base base) (arrow base base)) :=
-λ ν, lam (λ f, var f)
-
-#eval to_string i_nat
-#eval to_string $ term.normalize i_nat
-
-instance : setoid (Term Γ t) :=
-⟨inv_image eq term.normalize,
- inv_image.equivalence eq term.normalize eq.equivalence⟩
-
-def term.one : Term [] (arrow (arrow base base) (arrow base base)) :=
-λ ν, lam (λ f, lam (λ x, app (var f) (var x)))
-
-lemma zero_approx_zero : term.zero ≈ term.zero :=
-by reflexivity
-
-lemma succ_zero_approx_one : term.app term.succ term.zero ≈ term.one :=
-begin
-  unfold has_equiv.equiv setoid.r inv_image,
-  reflexivity
-end
+end stlc
